git/abentkamp/duper/Duper/Clause.lean
@@ -1,0 +1,189 @@
+import Lean
+import Duper.Util.Misc
+import Duper.Expr
+import Duper.Order
+
+namespace Duper
+open Lean
+open Lean.Meta
+
+structure Lit where
+  sign : Bool
+  lvl : Level
+  ty : Expr
+  lhs : Expr
+  rhs : Expr
+deriving Inhabited, BEq, Hashable
+
+inductive LitSide | lhs | rhs
+deriving Inhabited, BEq, Hashable
+
+structure LitPos where
+  side : LitSide
+  pos : ExprPos
+deriving Inhabited, BEq, Hashable
+
+
+namespace Lit
+
+def toExpr (lit : Lit) : Expr :=
+  if lit.sign
+  then mkApp3 (mkConst ``Eq [lit.lvl]) lit.ty lit.lhs lit.rhs
+  else mkApp3 (mkConst ``Ne [lit.lvl]) lit.ty lit.lhs lit.rhs
+
+def fromExpr (e : Expr) (sign := true) : Lit :=
+  Lit.mk
+    (sign := true)
+    (lvl := levelOne)
+    (ty := mkSort levelZero)
+    (lhs := e)
+    (rhs := if sign then mkConst ``True else mkConst ``False)
+
+def map (f : Expr → Expr) (l : Lit) :=
+  {l with ty := f l.ty, lhs := f l.lhs, rhs := f l.rhs}
+
+def mapM {m : Type → Type w} [Monad m] (f : Expr → m Expr) (l : Lit) : m Lit := do
+  return {l with ty := ← f l.ty, lhs := ← f l.lhs, rhs := ← f l.rhs}
+
+def fold {α : Type v} (f : α → Expr → α) (init : α) (l : Lit) : α :=
+  f (f (f init l.ty) l.lhs) l.rhs
+
+def foldWithTypeM {β : Type v} {m : Type v → Type w} [Monad m] 
+    (f : β → Expr → m β) (init : β) (l : Lit) : m β := do
+  f (← f (← f init l.ty) l.lhs) l.rhs
+
+def foldM {β : Type v} {m : Type v → Type w} [Monad m] 
+    (f : β → Expr → LitPos → m β) (init : β) (l : Lit) : m β := do
+  f (← f init l.lhs ⟨LitSide.lhs, ExprPos.empty⟩) l.rhs ⟨LitSide.rhs, ExprPos.empty⟩
+
+def foldGreenM {β : Type v} [Inhabited β] {m : Type v → Type w} [Monad m] 
+    (f : β → Expr → LitPos → m β) (init : β) (l : Lit) : m β := do
+  let fLhs := fun acc e p => f acc e ⟨LitSide.lhs, p⟩
+  let fRhs := fun acc e p => f acc e ⟨LitSide.rhs, p⟩
+  l.rhs.foldGreenM fRhs (← l.lhs.foldGreenM fLhs init) 
+
+def getAtPos! (l : Lit) (pos : LitPos) : Expr :=
+  match pos.side with
+  | LitSide.lhs => l.lhs.getAtPos! pos.pos
+  | LitSide.rhs => l.rhs.getAtPos! pos.pos
+
+def symm (l : Lit) : Lit :=
+{l with 
+  lhs := l.rhs
+  rhs := l.lhs}
+
+def makeLhs (lit : Lit) (side : LitSide) := match side with
+| LitSide.lhs => lit
+| LitSide.rhs => lit.symm
+
+def getSide (lit : Lit) (side : LitSide) := match side with
+| LitSide.lhs => lit.lhs
+| LitSide.rhs => lit.rhs
+
+instance : ToFormat Lit :=
+⟨ fun lit => format lit.toExpr ⟩
+
+instance : ToMessageData Lit :=
+⟨ fun lit => lit.toExpr ⟩
+
+
+open Comparison
+def compare (ord : Expr → Expr → MetaM Comparison) (l₁ l₂ : Lit) : MetaM Comparison := do
+  let cll ← ord l₁.lhs l₂.lhs
+  if cll == Incomparable then return Incomparable
+  let clr ← ord l₁.lhs l₂.rhs
+  if clr == Incomparable then return Incomparable
+  let crl ← ord l₁.rhs l₂.lhs
+  if crl == Incomparable then return Incomparable
+  let crr ← ord l₁.rhs l₂.rhs
+  if crr == Incomparable then return Incomparable
+
+  match cll, clr, crl, crr with
+  | GreaterThan, GreaterThan, _, _ => return GreaterThan
+  | _, _, GreaterThan, GreaterThan => return GreaterThan
+  | LessThan, _, LessThan, _ => return LessThan
+  | _, LessThan, _, LessThan => return LessThan
+
+  | GreaterThan, _, _, GreaterThan => return GreaterThan
+  | LessThan, _, _, LessThan => return LessThan
+  | _, GreaterThan, GreaterThan, _ => return GreaterThan
+  | _, LessThan, LessThan, _ => return LessThan
+  | _, _, _, _ => do
+
+    let csign := match l₁.sign, l₂.sign with
+    | true, true => Equal
+    | false, true => GreaterThan
+    | true, false => LessThan
+    | false, false => Equal
+
+    match cll, clr, crl, crr, csign with
+    | Equal, _, _, c, Equal => return c
+    | _, Equal, c, _, Equal => return c
+    | _, c, Equal, _, Equal => return c
+    | c, _, _, Equal, Equal => return c
+
+    | Equal, _, _, Equal, _ => return Equal
+    | _, Equal, Equal, _, _ => return Equal
+    
+    | Equal, _, _, _, c => return c
+    | _, Equal, _, _, c => return c
+    | _, _, Equal, _, c => return c
+    | _, _, _, Equal, c => return c
+
+    | _, _, _, _, _ => throwError "unexpected comparisons : {cll} {clr} {crl} {crr} {csign}"
+
+end Lit
+
+structure Clause :=
+(bVarTypes : Array Expr)
+(lits : Array Lit)
+deriving Inhabited, BEq, Hashable
+
+structure ClausePos where
+  lit : Nat
+  side : LitSide
+  pos : ExprPos
+deriving Inhabited, BEq, Hashable
+
+namespace Clause
+
+def empty : Clause := ⟨#[], #[]⟩
+
+def fromExpr (e : Expr) : Clause :=
+  Clause.mk #[] #[Lit.fromExpr e]
+
+def toExpr (c : Clause) : Expr :=
+  litsToExpr c.lits.data
+where litsToExpr : List Lit → Expr
+| [] => mkConst ``False
+| [l] => l.toExpr
+| l :: ls => mkApp2 (mkConst ``Or) l.toExpr (litsToExpr ls)
+
+def toForallExpr (c : Clause) : Expr :=
+  c.bVarTypes.foldr (fun ty b => mkForall Name.anonymous BinderInfo.default ty b) c.toExpr
+
+instance : ToFormat Clause :=
+⟨ fun c => format c.toExpr ⟩
+
+instance : ToMessageData Clause :=
+⟨ fun c => c.toExpr ⟩
+
+def weight (c : Clause) : Nat :=
+  c.lits.foldl (fun acc lit => acc + weightExpr lit.lhs + weightExpr lit.rhs) 0
+where 
+  weightExpr : Expr → Nat
+  | Expr.bvar _ _        => 1
+  | Expr.fvar _ _        => 1
+  | Expr.mvar _ _        => 1
+  | Expr.sort _ _        => 1
+  | Expr.const _ _ _     => 1
+  | Expr.app a b _       => weightExpr a + weightExpr b
+  | Expr.lam _ _ b _     => 1 + weightExpr b
+  | Expr.forallE _ _ b _ => 1 + weightExpr b
+  | Expr.letE _ _ v b _  => 1 + weightExpr v + weightExpr b
+  | Expr.lit _ _         => 1
+  | Expr.mdata _ b _     => 1 + weightExpr b
+  | Expr.proj _ _ b _    => 1 + weightExpr b
+
+end Clause
+
