git/abentkamp/duper/Duper/MClause.lean
@@ -1,0 +1,63 @@
+
+import Duper.Clause
+
+namespace Duper
+open Lean
+
+structure MClause :=
+(lits : Array Lit)
+deriving Inhabited, BEq, Hashable
+
+namespace MClause
+
+def appendLits (c : MClause) (lits : Array Lit) : MClause :=
+  ⟨c.lits.append lits⟩
+
+def eraseLit (c : MClause) (idx : Nat) : MClause :=
+  ⟨c.lits.eraseIdx idx⟩
+
+def mapM {m : Type → Type w} [Monad m] (f : Expr → m Expr) (c : MClause) : m MClause := do
+  return ⟨← c.lits.mapM (fun l => l.mapM f)⟩
+
+def foldM {β : Type v} {m : Type v → Type w} [Monad m] 
+    (f : β → Expr → ClausePos → m β) (init : β) (c : MClause) : m β := do
+  let mut acc := init
+  for i in [:c.lits.size] do
+    let f' := fun acc e pos => f acc e ⟨i, pos.side, pos.pos⟩
+    acc ← c.lits[i].foldM f' acc
+  return acc
+
+def foldGreenM {β : Type v} [Inhabited β] {m : Type v → Type w} [Monad m] 
+    (f : β → Expr → ClausePos → m β) (init : β) (c : MClause) : m β := do
+  let mut acc := init
+  for i in [:c.lits.size] do
+    let f' := fun acc e pos => f acc e ⟨i, pos.side, pos.pos⟩
+    acc ← c.lits[i].foldGreenM f' acc
+  return acc
+
+def getAtPos! (c : MClause) (pos : ClausePos) : Expr :=
+  c.lits[pos.lit].getAtPos! ⟨pos.side, pos.pos⟩
+
+def append (c : MClause) (d : MClause) : MClause := ⟨c.lits.append d.lits⟩
+
+def eraseIdx (i : Nat) (c : MClause) : MClause := ⟨c.lits.eraseIdx i⟩
+
+def isTrivial (c : MClause) : Bool := Id.run do
+  -- TODO: Also check if it contains the same literal positively and negatively?
+  for lit in c.lits do
+    if lit.sign ∧ lit.lhs == lit.rhs then
+      return true
+  return false
+
+open Comparison
+def isMaximalLit (ord : Expr → Expr → MetaM Comparison) (c : MClause) (idx : Nat) (strict := false): MetaM Bool := do
+  for j in [:c.lits.size] do
+    if j == idx then continue
+    let c ← Lit.compare ord c.lits[idx] c.lits[j]
+    if c == GreaterThan ∨ (¬ strict ∧ c == Equal)
+      then continue
+    else return false
+  return true
+
+end MClause
+end Duper
