git/abentkamp/duper/Duper/Order.lean
@@ -1,0 +1,146 @@
+import Lean
+
+namespace Duper
+open Lean
+
+inductive Comparison
+| GreaterThan
+| LessThan
+| Equal
+| Incomparable
+deriving BEq
+
+namespace Comparison
+
+instance : ToMessageData Comparison := ⟨
+  fun c => match c with
+| GreaterThan => ">"
+| LessThan => "<"
+| Equal => "="
+| Incomparable => "?"
+⟩ 
+
+end Comparison
+
+namespace Order
+open Lean.Meta
+open Comparison
+
+partial def weight (s : Expr) (w : Int := 0) (sign : Int) : MetaM Int := do
+  Core.checkMaxHeartbeats "weight"
+  trace[Meta.debug] "s: {s}" 
+  s.withApp fun f ss =>
+    match f with
+    | Expr.fvar .. => do
+      let mut w := w + sign * 1
+      for u in ss do
+        w ← weight u w sign
+      return w
+    | Expr.const .. => do
+      let mut w := w + sign * 1
+      for u in ss do
+        w ← weight u w sign
+      return w
+    | Expr.forallE _ _ body _ => do -- TODO: Also search type? 
+      let mut w := w + sign * 1
+      w ← weight body w sign
+      -- TODO: Assert ss empty?
+      return w
+    | Expr.bvar .. => do
+      let mut w := w + sign * 1
+      for u in ss do
+        w ← weight u w sign
+      return w
+    | Expr.sort .. => do
+      return w + sign * 1
+    | Expr.mvar mVarId .. => do
+      return w + sign * 1
+    | _ => throwError "Not implemented {s}"
+
+partial def varBalance (s : Expr) (vb : Std.HashMap Expr Int := {}) (sign : Int) : MetaM (Std.HashMap Expr Int) := do
+  Core.checkMaxHeartbeats "varBalance"
+  trace[Meta.debug] "s: {s}" 
+  s.withApp fun f ss =>
+    match f with
+    | Expr.fvar .. => do
+      let mut vb := vb
+      for u in ss do
+        vb ← varBalance u vb sign
+      return vb
+    | Expr.const .. => do
+      let mut vb := vb
+      for u in ss do
+        vb ← varBalance u vb sign
+      return vb
+    | Expr.forallE _ _ body _ => do -- TODO: Also search type?
+      let vb ← varBalance body vb sign
+      -- TODO: Assert ss empty?
+      return vb
+    | Expr.bvar .. => do
+      let mut vb := vb
+      for u in ss do
+        vb ← varBalance u vb sign
+      return vb
+    | Expr.sort .. => do
+      return vb
+    | Expr.mvar mVarId .. => do
+      let vb := vb.insert s $ vb.findD s 0 + sign
+      return vb
+    | _ => throwError "Not implemented {s}"
+
+def compareVarBalance (vb : Std.HashMap Expr Int := {}) : MetaM Comparison := do
+  let mut res := Equal
+  for (v, b) in vb.toArray do
+    if b > 0 then
+      if res == LessThan then
+        res := Incomparable
+        break
+      else
+        res := GreaterThan
+    else if b < 0 then
+      if res == GreaterThan then
+        res := Incomparable
+        break
+      else
+        res := LessThan
+  return res
+
+-- TODO: Not quite KBO yet
+def kbo (s t : Expr) : MetaM Comparison := do
+  Core.checkMaxHeartbeats "kbo"
+  if s == t then return Equal
+  else
+    let wb : Int := 0
+    let wb ← weight s wb 1
+    let wb ← weight t wb (-1)
+    let vb := {}
+    let vb ← varBalance s vb 1
+    let vb ← varBalance t vb (-1)
+    trace[Meta.debug] "wb: {wb}"
+    trace[Meta.debug] "vb: {vb.toArray}"
+    let vbComparison ← compareVarBalance vb
+    return if wb > 0 ∧ (vbComparison == GreaterThan ∨ vbComparison == Equal) then
+      GreaterThan
+    else if wb < 0 ∧ (vbComparison == LessThan ∨ vbComparison == Equal) then
+      LessThan
+    else
+      Incomparable
+
+
+def test : MetaM Unit := do
+  let ty := mkConst ``Nat
+  let x ← mkFreshExprMVar ty
+  let y ← mkFreshExprMVar ty
+  let s := (mkConst ``Nat.zero)
+  let t := mkApp (mkConst ``Nat.succ) x
+  let res ← kbo s t
+  trace[Meta.debug] "s: {s}"
+  trace[Meta.debug] "t: {t}"
+  trace[Meta.debug] "res: {res}"
+
+set_option trace.Meta.debug true
+#eval test
+
+end Order
+
+end Duper
