git/abentkamp/duper/Duper/ProverM.lean
@@ -1,0 +1,274 @@
+import Duper.Clause
+import Std.Data.BinomialHeap
+import Duper.DiscrTree
+import Duper.Selection
+
+namespace Duper
+namespace ProverM
+open Lean
+open Lean.Core
+open Std
+open RuleM
+
+inductive Result :=
+| unknown
+| saturated
+| contradiction
+  deriving Inhabited
+
+open Result
+
+structure ClauseInfo where
+(number : Nat)
+(proof : Proof)
+
+abbrev ClauseSet := HashSet Clause 
+abbrev ClauseHeap := BinomialHeap (Nat × Clause) fun c d => c.1 ≤ d.1
+abbrev ClauseDiscrTree α := Duper.DiscrTree (Clause × α)
+
+instance : ToMessageData Result := 
+⟨fun r => match r with
+| unknown => "unknown"
+| saturated => "saturated"
+| contradiction => "contradiction"⟩
+
+structure Context where
+  blah : Bool := false
+deriving Inhabited
+
+structure State where
+  result : Result := unknown
+  allClauses : HashMap Clause ClauseInfo := {}
+  activeSet : ClauseSet := {} --TODO: put clause into only in allClauses?
+  passiveSet : ClauseSet := {}
+  passiveSetAgeHeap : ClauseHeap := BinomialHeap.empty
+  passiveSetWeightHeap : ClauseHeap := BinomialHeap.empty
+  fairnessCounter : Nat := 0
+  supMainPremiseIdx : ClauseDiscrTree ClausePos := {}
+  supSidePremiseIdx : ClauseDiscrTree ClausePos := {}
+  lctx : LocalContext := {}
+
+abbrev ProverM := ReaderT Context $ StateRefT State CoreM
+
+instance : MonadLCtx ProverM where
+  getLCtx := return (← get).lctx
+
+instance : AddMessageContext ProverM where
+  addMessageContext := fun msgData => do
+    let env ← getEnv
+    let lctx ← getLCtx
+    let opts ← getOptions
+    pure $ MessageData.withContext { env := env, mctx := {}, lctx := lctx, opts := opts } msgData
+
+@[inline] def ProverM.run (x : ProverM α) (ctx : Context := {}) (s : State := {}) : CoreM (α × State) :=
+  x ctx |>.run s
+
+@[inline] def ProverM.run' (x : ProverM α) (ctx : Context := {}) (s : State := {}) : CoreM α :=
+  Prod.fst <$> x.run ctx s
+
+@[inline] def ProverM.toIO (x : ProverM α) (ctxCore : Core.Context) (sCore : Core.State) (ctx : Context := {}) (s : State := {}) : IO (α × Core.State × State) := do
+  let ((a, s), sCore) ← (x.run ctx s).toIO ctxCore sCore
+  pure (a, sCore, s)
+
+instance [MetaEval α] : MetaEval (ProverM α) :=
+  ⟨fun env opts x _ => MetaEval.eval env opts x.run' true⟩
+
+initialize
+  registerTraceClass `Prover
+  registerTraceClass `Prover.saturate
+  registerTraceClass `Prover.debug
+
+def getBlah : ProverM Bool :=
+  return (← read).blah
+
+def getResult : ProverM Result :=
+  return (← get).result
+
+def getAllClauses : ProverM (HashMap Clause ClauseInfo) :=
+  return (← get).allClauses
+
+def getActiveSet : ProverM ClauseSet :=
+  return (← get).activeSet
+
+def getPassiveSet : ProverM ClauseSet :=
+  return (← get).passiveSet
+
+def getPassiveSetAgeHeap : ProverM ClauseHeap :=
+  return (← get).passiveSetAgeHeap
+
+def getPassiveSetWeightHeap : ProverM ClauseHeap :=
+  return (← get).passiveSetWeightHeap
+
+def getFairnessCounter : ProverM Nat :=
+  return (← get).fairnessCounter
+
+def getSupMainPremiseIdx : ProverM (ClauseDiscrTree ClausePos) :=
+  return (← get).supMainPremiseIdx
+
+def getSupSidePremiseIdx : ProverM (ClauseDiscrTree ClausePos) :=
+  return (← get).supSidePremiseIdx
+
+def getClauseInfo! (c : Clause) : ProverM ClauseInfo := do
+  let some ci := (← getAllClauses).find? c
+    | throwError "Clause not found: {c}"
+  return ci
+
+def setResult (result : Result) : ProverM Unit :=
+  modify fun s => { s with result := result }
+
+def setActiveSet (activeSet : ClauseSet) : ProverM Unit :=
+  modify fun s => { s with activeSet := activeSet }
+
+def setAllClauses (allClauses : HashMap Clause ClauseInfo) : ProverM Unit :=
+  modify fun s => { s with allClauses := allClauses }
+
+def setPassiveSet (passiveSet : ClauseSet) : ProverM Unit :=
+  modify fun s => { s with passiveSet := passiveSet }
+
+def setPassiveSetAgeHeap (passiveSetAgeHeap : ClauseHeap) : ProverM Unit :=
+  modify fun s => { s with passiveSetAgeHeap := passiveSetAgeHeap }
+
+def setPassiveSetWeightHeap (passiveSetWeightHeap : ClauseHeap) : ProverM Unit :=
+  modify fun s => { s with passiveSetWeightHeap := passiveSetWeightHeap }
+
+def setFairnessCounter (fairnessCounter : Nat) : ProverM Unit :=
+  modify fun s => { s with fairnessCounter := fairnessCounter }
+
+def setSupSidePremiseIdx (supSidePremiseIdx : (ClauseDiscrTree ClausePos)) : ProverM Unit :=
+  modify fun s => { s with supSidePremiseIdx := supSidePremiseIdx }
+
+def setSupMainPremiseIdx (supMainPremiseIdx : (ClauseDiscrTree ClausePos)) : ProverM Unit :=
+  modify fun s => { s with supMainPremiseIdx := supMainPremiseIdx }
+
+def setLCtx (lctx : LocalContext) : ProverM Unit :=
+  modify fun s => { s with lctx := lctx }
+
+initialize emptyClauseExceptionId : InternalExceptionId ← registerInternalExceptionId `emptyClause
+
+def throwEmptyClauseException : ProverM α :=
+  throw <| Exception.internal emptyClauseExceptionId
+
+partial def chooseGivenClause : ProverM (Option Clause) := do
+  Core.checkMaxHeartbeats "chooseGivenClause"
+  -- Decide which heap to choose from
+  let fc ← getFairnessCounter
+  let (getHeap, setHeap) ←
+    if fc ≥ 5 then
+      setFairnessCounter 0
+      trace[Prover.debug] "Clause selected by age ({fc})"
+      pure (getPassiveSetAgeHeap, setPassiveSetAgeHeap)
+    else
+      trace[Prover.debug] "Clause selected by weight ({fc})"
+      pure (getPassiveSetWeightHeap, setPassiveSetWeightHeap)
+  -- Extract clause from heap
+  let some (c, h) := (← getHeap).deleteMin
+    | return none
+  setHeap h
+  -- If selected clause is no longer in passive set, restart.
+  if not $ (← getPassiveSet).contains c.2 then
+    return (← chooseGivenClause)
+  -- Remove clause from passive
+  setPassiveSet $ (← getPassiveSet).erase c.2
+  -- Increase fairness counter
+  setFairnessCounter (fc + 1)
+  return c.2
+
+/-- Registers a new clause, but does not add it to active or passive set.
+  Typically, you'll want to use `addNewToPassive` instead. -/
+def addNewClause (c : Clause) (proof : Proof) : ProverM ClauseInfo := do
+  match (← getAllClauses).find? c with
+  | some ci => return ci
+  | none =>
+    let allClauses := (← get).allClauses
+    let ci : ClauseInfo := {
+      number := allClauses.size
+      proof := proof
+    }
+    setAllClauses (allClauses.insert c ci)
+    if c.lits.size == 0 then throwEmptyClauseException
+    return ci
+
+def addNewToPassive (c : Clause) (proof : Proof) : ProverM Unit := do
+  if (← getAllClauses).contains c
+  then pure () -- clause is not new, ignore.
+  else
+    trace[Prover.saturate] "New passive clause: {c}"
+    let ci ← addNewClause c proof
+    setPassiveSet $ (← getPassiveSet).insert c
+    setPassiveSetAgeHeap $ (← getPassiveSetAgeHeap).insert (ci.number, c)
+    setPassiveSetWeightHeap $ (← getPassiveSetWeightHeap).insert (c.weight, c)
+
+def addExprAssumptionToPassive (e : Expr) (proof : Expr) : ProverM Unit := do
+  let c := Clause.fromExpr e
+  -- TODO: remove sorry
+  let mkProof := fun _ _ _ => pure proof
+  addNewToPassive c {ruleName := "assumption", mkProof := mkProof}
+  
+def ProverM.runWithExprs (x : ProverM α) (es : Array (Expr × Expr)) (ctx : Context := {}) (s : State := {}) : 
+    CoreM (α × State) := do
+  ProverM.run (s := s) (ctx := ctx) do
+    for (e, proof) in es do
+      addExprAssumptionToPassive e proof
+    x
+
+@[inline] def runRuleM (x : RuleM α) : ProverM.ProverM α := do
+  let (res, state) ← RuleM.run x (s := {lctx := ← getLCtx})
+  ProverM.setLCtx state.lctx
+  return res
+
+@[inline] def runInferenceRule (x : RuleM Unit) : ProverM.ProverM (Array (Clause × Proof)) := do
+  let (res, state) ← RuleM.run x (s := {lctx := ← getLCtx})
+  ProverM.setLCtx state.lctx
+  return state.resultClauses
+
+@[inline] def runSimpRule (x : RuleM α) : 
+    ProverM.ProverM (α × Array (Clause × Proof)) := do
+  let (res, state) ← RuleM.run x (s := {lctx := ← getLCtx})
+  ProverM.setLCtx state.lctx
+  return (res, state.resultClauses)
+
+def performInference (rule : MClause → RuleM Unit) (c : Clause) : ProverM Unit := do
+  let cs ← runInferenceRule do
+    let c ← loadClause c
+    rule c
+  for (c, proof) in cs do
+    addNewToPassive c proof
+
+def addToActive (c : Clause) : ProverM Unit := do
+  let ci ← getClauseInfo! c
+  --TODO: use event listeners for this?
+  -- Add to side premise index:
+  let idx ← getSupSidePremiseIdx
+  let idx ← runRuleM do
+    let (mvars, mclause) ← loadClauseCore c
+    mclause.foldM
+      fun idx e pos => do
+        if mclause.lits[pos.lit].sign ∧ litSelectedOrNothingSelected mclause pos.lit
+        then return ← idx.insert e (c, pos)
+        else return idx
+      idx
+  setSupSidePremiseIdx idx
+  -- Add to main premise index:
+  let idx ← getSupMainPremiseIdx
+  let idx ← runRuleM do
+    let (mvars, mclause) ← loadClauseCore c
+    mclause.foldGreenM
+      fun idx e pos => do
+        if e.isMVar
+        then return idx
+        else return ← idx.insert e (c, pos)
+      idx
+  setSupMainPremiseIdx idx
+  -- add to active set:
+  setActiveSet $ (← getActiveSet).insert c
+
+def mkFreshFVarId (ty : Expr): ProverM FVarId := do
+  let lctx ← getLCtx
+  let n := lctx.decls.size
+  let name := Name.mkNum `c n
+  let fVarId := ⟨name⟩
+  setLCtx $ LocalContext.mkLocalDecl lctx fVarId name ty
+  return fVarId
+
+end ProverM
+end Duper
