git/abentkamp/duper/Duper/RuleM.lean
@@ -1,0 +1,230 @@
+import Lean
+import Duper.Unif
+import Duper.MClause
+
+namespace Duper
+
+namespace RuleM
+open Lean
+open Lean.Core
+
+structure Context where
+  order : Expr → Expr → MetaM Comparison := Order.kbo
+deriving Inhabited
+
+structure ProofParent where
+  clause : Clause 
+  instantiations : Array Expr
+  vanishingVarTypes : Array Expr
+-- some variables disappear in inferences, 
+-- but need to be instantiated when reconstructing the proof
+-- e.g., EqRes on x != y
+deriving Inhabited
+
+/-- Takes: Proofs of the parent clauses, ProofParent information, the target clause -/
+abbrev ProofReconstructor := Array Expr → Array ProofParent → Clause → MetaM Expr
+
+structure Proof where
+  parents : Array ProofParent := #[]
+  ruleName : String := "unknown"
+  introducedSkolems : Array (FVarId × (Array Expr → MetaM Expr)) := #[]
+  mkProof : ProofReconstructor
+deriving Inhabited
+
+structure State where
+  mctx : MetavarContext := {}
+  lctx : LocalContext := {}
+  loadedClauses : Array (Clause × Array MVarId) := #[]
+  resultClauses : Array (Clause × Proof) := #[]
+  introducedSkolems : Array (FVarId × (Array Expr → MetaM Expr)) := #[]
+deriving Inhabited
+
+abbrev RuleM := ReaderT Context $ StateRefT State CoreM
+
+initialize
+  registerTraceClass `Rule
+  registerTraceClass `Rule.debug
+
+instance : MonadLCtx RuleM where
+  getLCtx := return (← get).lctx
+
+instance : MonadMCtx RuleM where
+  getMCtx    := return (← get).mctx
+  modifyMCtx f := modify fun s => { s with mctx := f s.mctx }
+
+@[inline] def RuleM.run (x : RuleM α) (ctx : Context := {}) (s : State := {}) : CoreM (α × State) :=
+  x ctx |>.run s
+
+@[inline] def RuleM.run' (x : RuleM α) (ctx : Context := {}) (s : State := {}) : CoreM α :=
+  Prod.fst <$> x.run ctx s
+
+@[inline] def RuleM.toIO (x : RuleM α) (ctxCore : Core.Context) (sCore : Core.State) (ctx : Context := {}) (s : State := {}) : IO (α × Core.State × State) := do
+  let ((a, s), sCore) ← (x.run ctx s).toIO ctxCore sCore
+  pure (a, sCore, s)
+
+instance [MetaEval α] : MetaEval (RuleM α) :=
+  ⟨fun env opts x _ => MetaEval.eval env opts x.run' true⟩
+
+def getOrder : RuleM (Expr → Expr → MetaM Comparison) :=
+  return (← read).order
+
+def getMCtx : RuleM MetavarContext :=
+  return (← get).mctx
+
+def getLoadedClauses : RuleM (Array (Clause × Array MVarId)) :=
+  return (← get).loadedClauses
+
+def getResultClauses : RuleM (Array (Clause × Proof)) :=
+  return (← get).resultClauses
+
+def getIntroducedSkolems : RuleM (Array (FVarId × (Array Expr → MetaM Expr))) :=
+  return (← get).introducedSkolems
+
+def setMCtx (mctx : MetavarContext) : RuleM Unit :=
+  modify fun s => { s with mctx := mctx }
+
+def setLCtx (lctx : LocalContext) : RuleM Unit :=
+  modify fun s => { s with lctx := lctx }
+
+def setLoadedClauses (loadedClauses : Array (Clause × Array MVarId)) : RuleM Unit :=
+  modify fun s => { s with loadedClauses := loadedClauses }
+
+def setResultClauses (resultClauses : Array (Clause × Proof)) : RuleM Unit :=
+  modify fun s => { s with resultClauses := resultClauses }
+
+def setIntroducedSkolems (introducedSkolems : Array (FVarId × (Array Expr → MetaM Expr))) : RuleM Unit :=
+  modify fun s => { s with introducedSkolems := introducedSkolems }
+
+def withoutModifyingMCtx (x : RuleM α) : RuleM α := do
+  let s ← getMCtx
+  try
+    x
+  finally
+    setMCtx s
+
+-- TODO: Reset `introducedSkolems`?
+def withoutModifyingLoadedClauses (x : RuleM α) : RuleM α := do
+  let s ← getLoadedClauses
+  try
+    withoutModifyingMCtx x
+  finally
+    setLoadedClauses s
+
+instance : AddMessageContext RuleM where
+  addMessageContext := addMessageContextFull
+
+
+-- TODO: MonadLift
+def runMetaAsRuleM (x : MetaM α) : RuleM α := do
+  let lctx ← getLCtx
+  let mctx ← getMCtx
+  let (res, state) ← Meta.MetaM.run (ctx := {lctx := lctx}) (s := {mctx := mctx}) do
+    x
+  setMCtx state.mctx
+  return res
+
+def mkFreshExprMVar (type? : Option Expr) (kind := MetavarKind.natural) (userName := Name.anonymous) : RuleM Expr := do
+  runMetaAsRuleM $ Meta.mkFreshExprMVar type? kind userName
+
+def getMVarType (mvarId : MVarId) : RuleM Expr := do
+  runMetaAsRuleM $ Meta.getMVarType mvarId
+
+def forallMetaTelescope (e : Expr) (kind := MetavarKind.natural) : RuleM (Array Expr × Array BinderInfo × Expr) :=
+  runMetaAsRuleM $ Meta.forallMetaTelescope e kind
+
+def mkFreshSkolem (name : Name) (type : Expr) (mkProof : Array Expr → MetaM Expr) : RuleM Expr := do
+  let name := Name.mkNum name (← getLCtx).decls.size
+  let (lctx, res) ← runMetaAsRuleM $ do
+    Meta.withLocalDeclD name type fun x => do
+      return (← getLCtx, x)
+  setLCtx lctx
+  setIntroducedSkolems $ (← getIntroducedSkolems).push (res.fvarId!, mkProof)
+  return res
+
+def mkForallFVars (xs : Array Expr) (e : Expr) (usedOnly : Bool := false) (usedLetOnly : Bool := true) : RuleM Expr :=
+  runMetaAsRuleM $ Meta.mkForallFVars xs e usedOnly usedLetOnly
+
+def inferType (e : Expr) : RuleM Expr :=
+  runMetaAsRuleM $ Meta.inferType e
+
+def instantiateMVars (e : Expr) : RuleM Expr :=
+  runMetaAsRuleM $ Meta.instantiateMVars e
+
+def unify (l : Array (Expr × Expr)) : RuleM Bool := do
+  runMetaAsRuleM $ Meta.unify l
+
+def isProof (e : Expr) : RuleM Bool := do
+  runMetaAsRuleM $ Meta.isProof e
+
+def isType (e : Expr) : RuleM Bool := do
+  runMetaAsRuleM $ Meta.isType e
+
+def getFunInfoNArgs (fn : Expr) (nargs : Nat) : RuleM Meta.FunInfo := do
+  runMetaAsRuleM $ Meta.getFunInfoNArgs fn nargs
+
+def replace (e : Expr) (target : Expr) (replacement : Expr) : RuleM Expr := do
+  Core.transform e (pre := fun s => 
+    return if s == target then TransformStep.done replacement else TransformStep.visit s )
+
+def loadClauseCore (c : Clause) : RuleM (Array Expr × MClause) := do
+  let mVars ← c.bVarTypes.mapM fun ty => mkFreshExprMVar (some ty)
+  let lits := c.lits.map fun l =>
+    l.map fun e => e.instantiateRev mVars
+  setLoadedClauses ((← getLoadedClauses).push (c, mVars.map Expr.mvarId!))
+  return (mVars, MClause.mk lits)
+
+def loadClause (c : Clause) : RuleM MClause := do
+  let (mvars, mclause) ← loadClauseCore c
+  return mclause
+
+def neutralizeMClauseCore (c : MClause) : RuleM (Clause × CollectMVars.State) := do
+  let c ← c |>.mapM instantiateMVars
+  let mVarIds := (c.lits.foldl (fun acc (l : Lit) =>
+    l.fold (fun acc e => e.collectMVars acc) acc) {})
+  let lits := c.lits.map fun l =>
+    l.map fun e => e.abstractMVars (mVarIds.result.map mkMVar)
+  let c := Clause.mk (← mVarIds.result.mapM getMVarType) lits
+  return (c, mVarIds)
+
+def neutralizeMClause (c : MClause) : RuleM Clause := do
+  return (← neutralizeMClauseCore c).1
+
+def yieldClauseCore (c : MClause) (ruleName : String) (mkProof : Option ProofReconstructor) : RuleM Unit := do
+  let (c, cVars) ← neutralizeMClauseCore c
+  let mut proofParents := #[]
+  for (loadedClause, instantiations) in ← getLoadedClauses do
+    let instantiations ← instantiations.mapM fun m => do instantiateMVars $ mkMVar m
+    let additionalVars := instantiations.foldl (fun acc e => e.collectMVars acc) 
+      {visitedExpr := cVars.visitedExpr, result := #[]} -- ignore vars in `cVars`
+    let instantiations := instantiations.map 
+      (fun e => e.abstractMVars ((cVars.result ++ additionalVars.result).map mkMVar))
+    proofParents := proofParents.push {
+      clause := loadedClause
+      instantiations := instantiations
+      vanishingVarTypes := ← additionalVars.result.mapM getMVarType
+    }
+  let mkProof := match mkProof with
+  | some mkProof => mkProof
+  | none => fun _ _ _ => 
+    -- TODO: Remove sorry!?
+    Lean.Meta.mkSorry c.toForallExpr (synthetic := true)
+  let proof := {
+    parents := proofParents,  
+    ruleName := ruleName,
+    introducedSkolems := ← getIntroducedSkolems --TODO: neutralize MVars?
+    mkProof := mkProof
+  }
+  setResultClauses ((← getResultClauses).push (c, proof))
+
+
+
+def yieldClause (c : MClause) (ruleName : String) (mkProof : Option ProofReconstructor := none) : RuleM Unit := do
+  let _ ← yieldClauseCore c ruleName mkProof
+
+def compare (s t : Expr) : RuleM Comparison := do
+  let ord ← getOrder
+  runMetaAsRuleM do ord s t
+
+end RuleM
+
+end Duper
