git/abentkamp/duper/Duper/Rules/Clausification.lean
@@ -1,0 +1,306 @@
+import Duper.MClause
+import Duper.RuleM
+import Duper.Simp
+import Duper.Util.ProofReconstruction
+
+namespace Duper
+open Lean
+open RuleM
+open SimpResult
+
+--TODO: move?
+theorem not_of_eq_false (h: p = False) : ¬ p := 
+  fun hp => h ▸ hp
+
+--TODO: move?
+theorem of_not_eq_false (h: (¬ p) = False) : p := 
+  Classical.byContradiction fun hn => h ▸ hn
+
+--TODO: move?
+theorem eq_true_of_not_eq_false (h : (¬ p) = False) : p = True := 
+  eq_true (of_not_eq_false h)
+
+--TODO: move?
+theorem eq_false_of_not_eq_true (h : (¬ p) = True) : p = False := 
+  eq_false (of_eq_true h)
+
+--TODO: move?
+theorem clausify_and_left (h : (p ∧ q) = True) : p = True := 
+  eq_true (of_eq_true h).left
+
+--TODO: move?
+theorem clausify_and_right (h : (p ∧ q) = True) : q = True := 
+  eq_true (of_eq_true h).right
+
+--TODO: move?
+theorem clausify_and_false (h : (p ∧ q) = False) : p = False ∨ q = False := by
+  apply @Classical.byCases p
+  · intro hp 
+    apply @Classical.byCases q
+    · intro hq
+      exact False.elim $ not_of_eq_false h ⟨hp, hq⟩
+    · intro hq
+      exact Or.intro_right _ (eq_false hq)
+  · intro hp
+    exact Or.intro_left _ (eq_false hp)
+
+--TODO: move?
+theorem clausify_or (h : (p ∨ q) = True) : p = True ∨ q = True := 
+  (of_eq_true h).elim 
+    (fun h => Or.intro_left _ (eq_true h))
+    (fun h => Or.intro_right _ (eq_true h))
+
+--TODO: move?
+theorem clausify_or_false_left (h : (p ∨ q) = False) : p = False := 
+  eq_false fun hp => not_of_eq_false h (Or.intro_left _ hp)
+
+--TODO: move?
+theorem clausify_or_false_right (h : (p ∨ q) = False) : q = False := 
+  eq_false fun hp => not_of_eq_false h (Or.intro_right _ hp)
+
+--TODO: move?
+theorem clausify_not (h : (¬ p) = True) : p = False := 
+eq_false fun hp => of_eq_true h hp
+
+--TODO: move?
+theorem clausify_not_false (h : (¬ p) = False) : p = True := 
+eq_true (Classical.byContradiction fun hp => not_of_eq_false h hp)
+
+--TODO: move?
+theorem clausify_imp (h : (p → q) = True) : (¬ p) = True ∨ q = True := 
+  (Classical.em q).elim 
+    (fun hq => Or.intro_right _ (eq_true hq)) 
+    (fun hq => Or.intro_left _ (eq_true (fun hp => hq ((of_eq_true h) hp))))
+
+--TODO: move?
+theorem clausify_imp_false_left (h : (p → q) = False) : p = True := 
+  Classical.byContradiction fun hnp => 
+    not_of_eq_false h fun hp => 
+      False.elim (hnp $ eq_true hp)
+
+--TODO: move?
+theorem clausify_imp_false_right (h : (p → q) = False) : q = False := 
+  eq_false fun hq => not_of_eq_false h fun _ => hq
+
+--TODO: move?
+theorem clausify_forall {p : α → Prop} (x : α) (h : (∀ x, p x) = True) : p x = True := 
+  eq_true (of_eq_true h x)
+
+--TODO: move?
+theorem clausify_exists {p : α → Prop} (h : (∃ x, p x) = True) :
+  p (Classical.choose (of_eq_true h)) = True := 
+eq_true $ Classical.choose_spec _
+
+--TODO: move?
+theorem clausify_exists_false {p : α → Prop} (x : α) (h : (∃ x, p x) = False) : p x = False := 
+  eq_false (fun hp => not_of_eq_false h ⟨x, hp⟩)
+
+--TODO: move
+noncomputable def Inhabited.some [Inhabited α] (p : α → Prop) :=
+  let _ : Decidable (∃ a, p a) := Classical.propDecidable _
+  if hp: ∃ a, p a then Classical.choose hp else Inhabited.default
+
+--TODO: move
+theorem Inhabited.some_spec [Inhabited α] {p : α → Prop} (hp : ∃ a, p a) : 
+  p (Inhabited.some p) := by
+  simp only [Inhabited.some, hp]
+  exact Classical.choose_spec _
+
+theorem exists_of_forall_eq_false {p : α → Prop} (h : (∀ x, p x) = False) : ∃ x, ¬ p x := by
+  apply Classical.byContradiction
+  intro hnex
+  apply not_of_eq_false h
+  intro x
+  apply Classical.byContradiction
+  intro hp
+  apply hnex
+  exact Exists.intro x hp
+
+theorem false_neq_true : False ≠ True := fun h => of_eq_true h
+
+theorem true_neq_false : True ≠ False := fun h => of_eq_true h.symm
+
+-- TODO: Clausify ↔ as =
+def clausificationStepE (e : Expr) (sign : Bool) (c : MClause) (i : Nat) : 
+    RuleM (SimpResult (List (MClause × Option (Expr → MetaM Expr)))) := do
+  match sign, e with
+  | false, Expr.const ``True _ _ => do
+    let pr : Expr → MetaM Expr := fun premise => do
+      return ← Meta.mkAppM ``true_neq_false #[premise]
+    return Applied [(MClause.mk #[], some pr)]
+  | true, Expr.const ``False _ _ => do
+    let pr : Expr → MetaM Expr := fun premise => do
+      return ← Meta.mkAppM ``false_neq_true #[premise]
+    return Applied [(MClause.mk #[], some pr)]
+  | true, Expr.app (Expr.const ``Not _ _) e _ => do
+    let pr : Expr → MetaM Expr := fun premise => do
+      return ← Meta.mkAppM ``clausify_not #[premise]
+    return Applied [(MClause.mk #[Lit.fromExpr e false], some pr)]
+  | false, Expr.app (Expr.const ``Not _ _) e _ => 
+    let pr : Expr → MetaM Expr := fun premise => do
+      return ← Meta.mkAppM ``clausify_not_false #[premise]
+    return Applied [(MClause.mk #[Lit.fromExpr e true], some pr)]
+  | true, Expr.app (Expr.app (Expr.const ``And _ _) e₁ _) e₂ _ => do
+    let pr₁ : Expr → MetaM Expr := fun premise => do
+      return ← Meta.mkAppM ``clausify_and_left #[premise]
+    let pr₂ : Expr → MetaM Expr := fun premise => do
+      return ← Meta.mkAppM ``clausify_and_right #[premise]
+    return Applied [(MClause.mk #[Lit.fromExpr e₁], some pr₁), (MClause.mk #[Lit.fromExpr e₂], some pr₂)]
+  | true, Expr.app (Expr.app (Expr.const ``Or _ _) e₁ _) e₂ _ =>
+    let pr : Expr → MetaM Expr := fun premise => do
+      return ← Meta.mkAppM ``clausify_or #[premise]
+    return Applied [(MClause.mk #[Lit.fromExpr e₁, Lit.fromExpr e₂], some pr)]
+  | true, Expr.forallE _ ty b _ => do
+    if (← inferType ty).isProp
+    then
+      if b.hasLooseBVars then
+        throwError "Types depending on props are not supported" 
+      let pr : Expr → MetaM Expr := fun premise => do
+        return ← Meta.mkAppM ``clausify_imp #[premise]
+      return Applied [(MClause.mk #[Lit.fromExpr (mkNot ty), Lit.fromExpr b], some pr)]
+    else 
+      let mvar ← mkFreshExprMVar ty
+      let pr : Expr → MetaM Expr := fun premise => do
+        let mvar ← Meta.mkFreshExprMVar ty
+        return ← Meta.mkAppM ``clausify_forall #[mvar, premise]
+      return Applied [(MClause.mk #[Lit.fromExpr $ b.instantiate1 mvar], some pr)]
+  | true, Expr.app (Expr.app (Expr.const ``Exists _ _) ty _) (Expr.lam _ _ b _) _ => do
+    let skTerm ← makeSkTerm ty b
+    let pr : Expr → MetaM Expr := fun premise => do
+      return ← Meta.mkAppM ``eq_true
+        #[← Meta.mkAppM ``Inhabited.some_spec #[← Meta.mkAppM ``of_eq_true #[premise]]]
+    return Applied [(MClause.mk #[Lit.fromExpr $ b.instantiate1 skTerm], some pr)]
+  | false, Expr.app (Expr.app (Expr.const ``And _ _) e₁ _) e₂ _  => 
+    let pr : Expr → MetaM Expr := fun premise => do
+      return ← Meta.mkAppM ``clausify_and_false #[premise]
+    return Applied [(MClause.mk #[Lit.fromExpr e₁ false, Lit.fromExpr e₂ false], some pr)]
+  | false, Expr.app (Expr.app (Expr.const ``Or _ _) e₁ _) e₂ _ =>
+    let pr₁ : Expr → MetaM Expr := fun premise => do
+      return ← Meta.mkAppM ``clausify_or_false_left #[premise]
+    let pr₂ : Expr → MetaM Expr := fun premise => do
+      return ← Meta.mkAppM ``clausify_or_false_right #[premise]
+    return  Applied [(MClause.mk #[Lit.fromExpr e₁ false], some pr₁), 
+             (MClause.mk #[Lit.fromExpr e₂ false], some pr₂)]
+  | false, Expr.forallE _ ty b _ => do
+    if (← inferType ty).isProp
+    then 
+      if b.hasLooseBVars then
+        throwError "Types depending on props are not supported"
+      let pr₁ : Expr → MetaM Expr := fun premise => do
+        Meta.mkAppM ``clausify_imp_false_left #[premise]
+      let pr₂ : Expr → MetaM Expr := fun premise => do
+        Meta.mkAppM ``clausify_imp_false_right #[premise]
+      return Applied [(MClause.mk #[Lit.fromExpr ty], some pr₁),
+               (MClause.mk #[Lit.fromExpr b false], some pr₂)]
+    else
+      let skTerm ← makeSkTerm ty (mkNot b)
+      let pr : Expr → MetaM Expr := fun premise => do
+        Meta.mkAppM ``eq_true
+          #[← Meta.mkAppM ``Inhabited.some_spec #[← Meta.mkAppM ``exists_of_forall_eq_false #[premise]]]
+      return Applied [(MClause.mk #[Lit.fromExpr $ (mkNot b).instantiate1 skTerm], some pr)]
+  | false, Expr.app (Expr.app (Expr.const ``Exists _ _) ty _) (Expr.lam _ _ b _) _ => do
+    let mvar ← mkFreshExprMVar ty
+    let pr : Expr → MetaM Expr := fun premise => do
+      let mvar ← Meta.mkFreshExprMVar ty
+      Meta.mkAppM ``clausify_exists_false #[mvar, premise]
+    return Applied [(MClause.mk #[Lit.fromExpr (b.instantiate1 mvar) false], some pr)]
+  | true, Expr.app (Expr.app (Expr.app (Expr.const ``Eq [lvl] _) ty _) e₁ _) e₂ _  =>
+    let pr : Expr → MetaM Expr := fun premise => do
+      Meta.mkAppM ``of_eq_true #[premise]
+    return Applied [(MClause.mk #[{sign := true, lhs := e₁, rhs := e₂, lvl := lvl, ty := ty}], some pr)]
+  | false, Expr.app (Expr.app (Expr.app (Expr.const ``Eq [lvl] _) ty _) e₁ _) e₂ _  =>
+    let pr : Expr → MetaM Expr := fun premise => do
+      Meta.mkAppM ``not_of_eq_false #[premise] 
+    return Applied [(MClause.mk #[{sign := false, lhs := e₁, rhs := e₂, lvl := lvl, ty := ty}], some pr)]
+  | true, Expr.app (Expr.app (Expr.app (Expr.const ``Ne [lvl] _) ty _) e₁ _) e₂ _  =>
+    let pr : Expr → MetaM Expr := fun premise => do
+       Meta.mkAppM ``of_eq_true #[premise]
+    return Applied [(MClause.mk #[{sign := false, lhs := e₁, rhs := e₂, lvl := lvl, ty := ty}], some pr)]
+  | false, Expr.app (Expr.app (Expr.app (Expr.const ``Ne [lvl] _) ty _) e₁ _) e₂ _  =>
+    let pr : Expr → MetaM Expr := fun premise => do
+      Meta.mkAppM ``of_not_eq_false #[premise]
+    return Applied [(MClause.mk #[{sign := true, lhs := e₁, rhs := e₂, lvl := lvl, ty := ty}], some pr)]
+  | _, _ => return Unapplicable
+
+where
+  makeSkTerm ty b : RuleM Expr := do
+    let mVarIds := (e.collectMVars {}).result
+    let skTy := ty.abstractMVars (mVarIds.map mkMVar)
+    let mVarIdTys ← (mVarIds.mapM (fun mvarId => do inferType (mkMVar mvarId)))
+    let skTy := mVarIdTys.foldr
+      (fun mVarIdTy skTy => mkForall `_ BinderInfo.default mVarIdTy skTy)
+      skTy
+    let mkProof := fun parents => do
+      let d ← Meta.mkAppM ``Inhabited.some #[mkLambda `x BinderInfo.default ty b]
+      return d
+    let fvar ← mkFreshSkolem `sk skTy mkProof
+    return mkAppN fvar (mVarIds.map mkMVar)
+
+def clausificationStepLit (c : MClause) (i : Nat) : RuleM (SimpResult (List (MClause × Option (Expr → MetaM Expr)))) := do
+  let l := c.lits[i]
+  if not l.ty.isProp then return Unapplicable
+  if l.sign then
+    -- Clausify " = False" and "= True":
+    match l.rhs with
+    | Expr.const ``True _ _ => clausificationStepE l.lhs true c i
+    | Expr.const ``False _ _ => clausificationStepE l.lhs false c i
+    | _ => return Unapplicable
+  else
+    -- Clausify inequalities of type Prop:
+    return Applied [(MClause.mk #[Lit.fromExpr l.lhs false, Lit.fromExpr l.rhs false], none),
+             (MClause.mk #[Lit.fromExpr l.lhs true, Lit.fromExpr l.rhs true], none)]
+             -- TODO: Proofs
+-- TODO: True/False on left-hand side?
+
+-- TODO: generalize combination of `orCases` and `orIntro`?
+def clausificationStep : MSimpRule := fun c => do
+  for i in [:c.lits.size] do
+    match ← clausificationStepLit c i with
+    | Applied ds =>
+      return Applied $ ds.map fun (d, dproof) => 
+        let mkProof : ProofReconstructor := 
+          fun (premises : Array Expr) (parents: Array ProofParent) (res : Clause) => do
+            Meta.forallTelescope res.toForallExpr fun xs body => do
+              let resLits := res.lits.map (fun l => l.map (fun e => e.instantiateRev xs))
+              let (parentLits, appliedPremise) ← instantiatePremises parents premises xs
+              let parentLits := parentLits[0]
+              let appliedPremise := appliedPremise[0]
+              
+              let mut caseProofs := #[]
+              for j in [:parentLits.size] do
+                let lit := parentLits[j]
+                let pr ← Meta.withLocalDeclD `h lit.toExpr fun h => do
+                  if j == i then
+                    let resLeft := resLits.toList.take (c.lits.size - 1)
+                    let resRight := resLits.toList.drop (c.lits.size - 1)
+                    let resRight' := (Clause.mk #[] resRight.toArray).toForallExpr
+                    let resLits' := (resLeft.map Lit.toExpr).toArray.push resRight'
+                    -- TODO: use dproof and h
+                    let dproof ← match dproof with
+                    | none => Meta.mkSorry resRight' true
+                    | some dproof => dproof h
+                    if not (← Meta.isDefEq (← Meta.inferType dproof) resRight') then
+                      throwError "Error when reconstructing clausification. Expected type: {resRight'}, but got: {dproof}"
+                    if resRight.length == 0 then
+                      Meta.mkLambdaFVars #[h] $ ← Meta.mkAppOptM ``False.elim #[body, dproof]
+                    else
+                      Meta.mkLambdaFVars #[h] $ ← orIntro resLits' (c.lits.size - 1) dproof
+                  else
+                    let idx := if j ≥ i then j - 1 else j
+                    Meta.mkLambdaFVars #[h] $ ← orIntro (resLits.map Lit.toExpr) idx h
+                caseProofs := caseProofs.push $ pr
+
+              let r ← orCases (parentLits.map Lit.toExpr) caseProofs
+              trace[Meta.debug] "###RES {res}"
+              trace[Meta.debug] "###R {← Meta.inferType r}"
+              let r ← Meta.mkLambdaFVars xs $ mkApp r appliedPremise
+              trace[Meta.debug] "###R {r}"
+              return r
+        (⟨c.lits.eraseIdx i ++ d.lits⟩, mkProof)
+    | Removed => 
+      return Removed
+    | Unapplicable => 
+      continue
+  return Unapplicable
+
+end Duper
