git/abentkamp/duper/Duper/Rules/EqualityResolution.lean
@@ -1,0 +1,61 @@
+import Duper.ProverM
+import Duper.RuleM
+import Duper.MClause
+import Duper.Util.ProofReconstruction
+
+namespace Duper
+open RuleM
+open Lean
+
+def mkEqualityResolutionProof (i : Nat) (premises : Array Expr) (parents: Array ProofParent) (c : Clause) : MetaM Expr := do
+  let premise := premises[0]
+  let parent := parents[0]
+  Meta.forallTelescope c.toForallExpr fun xs body => do
+    let cLits := c.lits.map (fun l => l.map (fun e => e.instantiateRev xs))
+    let (parentsLits, appliedPremises) ← instantiatePremises parents premises xs
+    let parentLits := parentsLits[0]
+    let appliedPremise := appliedPremises[0]
+
+    let mut caseProofs := #[]
+    for j in [:parentLits.size] do
+      let lit := parentLits[j]
+      if j == i then
+        -- lit has the form t ≠ t
+        let pr ← Meta.withLocalDeclD `h lit.toExpr fun h => do
+          let pr := mkApp2 (mkConst ``rfl [lit.lvl]) lit.ty lit.lhs
+          let pr := mkApp h pr
+          let pr := mkApp2 (mkConst ``False.elim [levelZero]) body pr
+          Meta.mkLambdaFVars #[h] pr
+        caseProofs := caseProofs.push pr
+      else
+        -- need proof of `L_j → L_1 ∨ ... ∨ L_n`
+        let pr ← Meta.withLocalDeclD `h lit.toExpr fun h => do
+          let idx := if j ≥ i then j - 1 else j
+          Meta.mkLambdaFVars #[h] $ ← orIntro (cLits.map Lit.toExpr) idx h
+        -- caseProofs := caseProofs.push $ ← Lean.Meta.mkSorry (← Meta.mkArrow lit.toExpr body) (synthetic := true)
+        caseProofs := caseProofs.push $ pr
+
+    let r ← orCases (parentLits.map Lit.toExpr) caseProofs
+    Meta.mkLambdaFVars xs $ mkApp r appliedPremise
+
+def equalityResolutionAtLit (c : MClause) (i : Nat) : RuleM Unit :=
+  withoutModifyingMCtx $ do
+    let lit := c.lits[i]
+    if ← unify #[(lit.lhs, lit.rhs)]
+    then
+      let c := c.eraseLit i
+      yieldClause c "equality resolution" 
+        (mkProof := mkEqualityResolutionProof i)
+
+def equalityResolution (c : MClause) : RuleM Unit := do
+  for i in [:c.lits.size] do
+    if c.lits[i].sign = false ∧ litSelectedOrNothingSelected c i then
+      equalityResolutionAtLit c i
+
+open ProverM
+
+def performEqualityResolution (givenClause : Clause) : ProverM Unit := do
+  trace[Prover.debug] "EqRes inferences with {givenClause}"
+  performInference equalityResolution givenClause
+
+end Duper
