git/abentkamp/duper/Duper/Rules/Superposition.lean
@@ -1,0 +1,148 @@
+import Duper.ProverM
+import Duper.RuleM
+import Duper.Selection
+import Duper.Util.ProofReconstruction
+
+namespace Duper
+open RuleM
+open Lean
+
+-- TODO: Pass in the clauses later?
+def mkSuperpositionProof (sidePremiseLitIdx : Nat) (sidePremiseLitSide : LitSide) (givenIsMain : Bool) 
+    (premises : Array Expr) (parents: Array ProofParent) (c : Clause) : MetaM Expr := do
+  Meta.forallTelescope c.toForallExpr fun xs body => do
+    let cLits := c.lits.map (fun l => l.map (fun e => e.instantiateRev xs))
+    let (parentsLits, appliedPremises) ← instantiatePremises parents premises xs
+    
+    let mainParentLits := if givenIsMain then parentsLits[0] else parentsLits[1]
+    let sideParentLits := if givenIsMain then parentsLits[1] else parentsLits[0]
+    let appliedMainPremise := if givenIsMain then appliedPremises[0] else appliedPremises[1]
+    let appliedSidePremise := if givenIsMain then appliedPremises[1] else appliedPremises[0]
+
+    let mut caseProofsSide := #[]
+    for j in [:sideParentLits.size] do
+      if j == sidePremiseLitIdx then
+        let eqLit := sideParentLits[j]
+        let pr ← Meta.withLocalDeclD `heq eqLit.toExpr fun heq => do
+          let eq := if sidePremiseLitSide == LitSide.rhs 
+                      then ← Meta.mkAppM ``Eq.symm #[heq] 
+                      else heq
+          let mut caseProofsMain : Array Expr := #[]
+          for i in [:mainParentLits.size] do
+            let lit := mainParentLits[i]
+            let pr ← Meta.withLocalDeclD `h lit.toExpr fun h => do
+              let idx := sideParentLits.size - 1 + i
+              let abstr ← Meta.kabstract lit.toExpr $ eqLit.getSide sidePremiseLitSide
+              let abstr := mkLambda `x BinderInfo.default (← Meta.inferType eqLit.lhs) abstr
+              let rwproof ← Meta.mkAppM ``Eq.mp #[← Meta.mkAppM ``congrArg #[abstr,eq], h]
+              Meta.mkLambdaFVars #[h] $ ← orIntro (cLits.map Lit.toExpr) idx $ rwproof
+            caseProofsMain := caseProofsMain.push $ pr
+          let r ← orCases (mainParentLits.map Lit.toExpr) caseProofsMain
+          Meta.mkLambdaFVars #[heq] $ mkApp r appliedMainPremise
+        caseProofsSide := caseProofsSide.push $ pr
+      else
+        let lit := sideParentLits[j]
+        let pr ← Meta.withLocalDeclD `h lit.toExpr fun h => do
+          let idx := if j ≥ sidePremiseLitIdx then j - 1 else j
+          Meta.mkLambdaFVars #[h] $ ← orIntro (cLits.map Lit.toExpr) idx h
+        caseProofsSide := caseProofsSide.push $ pr
+
+    let r ← orCases (sideParentLits.map Lit.toExpr) caseProofsSide
+    let proof ← Meta.mkLambdaFVars xs $ mkApp r appliedSidePremise
+    -- Meta.mkLambdaFVars xs $ ← Lean.Meta.mkSorry body (synthetic := true)
+    return proof
+
+def superpositionAtLitWithPartner (mainPremise : MClause) (mainPremiseSubterm : Expr) 
+    (sidePremise : MClause) (sidePremiseLitIdx : Nat) (sidePremiseSide : LitSide) (givenIsMain : Bool): RuleM Unit := do
+  Core.checkMaxHeartbeats "superposition"
+  withoutModifyingMCtx $ do
+    let sidePremiseLit := sidePremise.lits[sidePremiseLitIdx].makeLhs sidePremiseSide
+    let restOfSidePremise := sidePremise.eraseIdx sidePremiseLitIdx
+    if mainPremiseSubterm.isMVar then
+      return ()
+    if not $ ← unify #[(mainPremiseSubterm, sidePremiseLit.lhs)] then
+      return ()
+    let lhs ← instantiateMVars sidePremiseLit.lhs
+    let rhs ← instantiateMVars sidePremiseLit.rhs
+    if (← compare lhs rhs) == Comparison.LessThan then
+      return ()
+
+    let sidePremise ← sidePremise.mapM fun e => instantiateMVars e
+    if not $ ← runMetaAsRuleM $ sidePremise.isMaximalLit (← getOrder) sidePremiseLitIdx then
+      return ()
+    -- TODO: make exception for selected lits
+
+    -- TODO: also check maximality for main premise
+
+    let mainPremiseReplaced ← 
+      mainPremise.mapM fun e => do
+        replace (← instantiateMVars e) lhs rhs --TODO: Replace only green subterms
+
+    -- if mainPremiseReplaced.isTrivial then
+    --   trace[Prover.debug] "trivial: {mainPremiseReplaced.lits}"
+      -- return ()
+      
+    let restOfSidePremise ← restOfSidePremise.mapM fun e => instantiateMVars e
+    let res := MClause.append restOfSidePremise mainPremiseReplaced 
+    yieldClause res "superposition" 
+      (mkProof := mkSuperpositionProof sidePremiseLitIdx sidePremiseSide givenIsMain)
+
+def superpositionAtLit (mainPremiseIdx : ProverM.ClauseDiscrTree ClausePos) 
+      (sidePremise : MClause) (sidePremiseLitIdx : Nat) (sidePremiseSide : LitSide) : 
+    RuleM Unit := do
+  let sidePremiseLit := sidePremise.lits[sidePremiseLitIdx].makeLhs sidePremiseSide
+  trace[Rule.debug] "Superposition inferences at literal {sidePremiseLit}"
+  let potentialPartners ← mainPremiseIdx.getUnify sidePremiseLit.lhs
+  -- trace[Rule.debug] "Potential partners {potentialPartners}"
+  for (partnerClause, partnerPos) in potentialPartners do
+    withoutModifyingLoadedClauses $ do
+      trace[Rule.debug] "Superposition with partner clause {partnerClause}"
+      let c ← loadClause partnerClause
+      superpositionAtLitWithPartner c (c.getAtPos! partnerPos)
+          sidePremise sidePremiseLitIdx sidePremiseSide (givenIsMain := false)
+
+def superpositionAtExpr (e : Expr) (sidePremiseIdx : ProverM.ClauseDiscrTree ClausePos)
+    (mainPremise : MClause) : RuleM Unit := do
+  trace[Rule.debug] "Superposition inferences at expression {e}"
+  let potentialPartners ← sidePremiseIdx.getUnify e
+  -- trace[Rule.debug] "Potential partners {potentialPartners}"
+  for (partnerClause, partnerPos) in potentialPartners do
+    withoutModifyingLoadedClauses $ do
+      trace[Rule.debug] "Superposition with partner clause {partnerClause}"
+      let c ← loadClause partnerClause
+      superpositionAtLitWithPartner mainPremise e
+          c partnerPos.lit partnerPos.side (givenIsMain := true)
+          
+
+def superposition 
+    (mainPremiseIdx : ProverM.ClauseDiscrTree ClausePos) 
+    (sidePremiseIdx : ProverM.ClauseDiscrTree ClausePos) 
+    (givenMClause : MClause) : RuleM Unit := do
+  -- With given clause as side premise:
+  -- trace[Rule.debug] "Superposition inferences with {givenClause} as side premise"
+  for i in [:givenMClause.lits.size] do
+    if givenMClause.lits[i].sign = true && litSelectedOrNothingSelected givenMClause i
+    then 
+      let restOfGivenClause := givenMClause.eraseIdx i
+      for side in #[LitSide.lhs, LitSide.rhs] do
+        let flippedLit := givenMClause.lits[i].makeLhs side
+        if (← RuleM.compare flippedLit.lhs flippedLit.rhs) == Comparison.LessThan then
+          continue
+        let cs ← superpositionAtLit mainPremiseIdx givenMClause i side
+  -- With given clause as main premise
+  -- trace[Rule.debug] "Superposition inferences with {givenClause} as main premise"
+  givenMClause.foldGreenM fun acc e pos => do
+      superpositionAtExpr e sidePremiseIdx givenMClause
+    ()
+  -- TODO: What about inference with itself?
+      
+open ProverM
+
+def performSuperposition (givenClause : Clause) : ProverM Unit := do
+  trace[Prover.debug] "Superposition inferences with {givenClause}"
+  let mainPremiseIdx ← getSupMainPremiseIdx
+  let sidePremiseIdx ← getSupSidePremiseIdx
+  performInference (superposition mainPremiseIdx sidePremiseIdx) givenClause
+
+
+end Duper
