git/abentkamp/duper/Duper/Rules/TrivialSimp.lean
@@ -1,0 +1,14 @@
+import Duper.Simp
+
+namespace Duper
+open RuleM
+open SimpResult
+
+-- TODO: Do this on Clause instead of MClause?
+def trivialSimp : MSimpRule := fun c => do
+  for lit in c.lits do
+    if lit.sign ∧ lit.lhs == lit.rhs then
+      return Removed
+  return Unapplicable
+
+end Duper
