git/abentkamp/duper/Duper/Saturate.lean
@@ -1,0 +1,92 @@
+import Duper.ProverM
+import Duper.Util.Iterate
+import Duper.RuleM
+import Duper.MClause
+import Duper.Rules.Clausification
+import Duper.Simp
+import Duper.Rules.Superposition
+import Duper.Rules.ClausifyPropEq
+import Duper.Rules.EqualityResolution
+import Duper.Rules.TrivialSimp
+import Duper.Rules.ElimDupLit
+import Std.Data.BinomialHeap
+
+namespace Duper
+
+namespace ProverM
+open Lean
+open Meta
+open Lean.Core
+open Result
+open Std
+open ProverM
+open RuleM
+
+set_option trace.Prover.debug true
+
+set_option maxHeartbeats 10000
+
+open SimpResult
+
+def simpRules := #[
+  (clausificationStep.toSimpRule, "clausification"),
+  (trivialSimp.toSimpRule, "trivial simp"),
+  (elimDupLit.toSimpRule, "eliminate duplicate literals")
+]
+
+def applySimpRules (givenClause : Clause) :
+    ProverM (SimpResult Clause) := do
+  for (simpRule, ruleName) in simpRules do
+    match ← simpRule ruleName givenClause with
+    | Removed => return Removed
+    | Applied c => return Applied c
+    | Unapplicable => continue
+  return Unapplicable
+
+partial def simpLoop (givenClause : Clause) : ProverM (Option Clause) := do
+  Core.checkMaxHeartbeats "simpLoop"
+  match ← applySimpRules givenClause with
+  | Applied c => 
+    simpLoop c
+  | Unapplicable => return some givenClause 
+  | Removed => return none
+
+def forwardSimplify (givenClause : Clause) : ProverM (Option Clause) := do
+  let c := simpLoop givenClause
+  -- TODO: Check for empty clause and raise throwEmptyClauseException
+  c
+
+def backwardSimplify (givenClause : Clause) : ProverM Unit := do
+  return ()
+
+def performInferences (givenClause : Clause) : ProverM Unit := do
+  performEqualityResolution givenClause
+  performClausifyPropEq givenClause
+  performSuperposition givenClause
+
+partial def saturate : ProverM Unit := do
+  Core.withCurrHeartbeats $ iterate $
+    try do
+      Core.checkMaxHeartbeats "saturate"
+      let some givenClause ← chooseGivenClause
+        | do
+          setResult saturated
+          return LoopCtrl.abort
+      trace[Prover.saturate] "### Given clause: {givenClause}"
+      let some givenClause ← forwardSimplify givenClause
+        | return LoopCtrl.next
+      trace[Prover.saturate] "### Given clause after simp: {givenClause}"
+      backwardSimplify givenClause
+      addToActive givenClause
+      performInferences givenClause
+      trace[Prover.saturate] "### New active Set: {(← getActiveSet).toArray}"
+      return LoopCtrl.next
+    catch
+    | Exception.internal emptyClauseExceptionId _  =>
+      setResult contradiction
+      return LoopCtrl.abort
+    | e => throw e
+
+end ProverM
+
+end Duper
