git/abentkamp/duper/Duper/Selection.lean
@@ -1,0 +1,20 @@
+import Duper.MClause
+
+namespace Duper
+open Lean
+
+-- TODO: Add simplification to always put True/False on right-hand side?
+def getSelections (c : MClause) : List Nat := Id.run do
+  -- simply select first negative literal:
+  for i in [:c.lits.size] do
+    if c.lits[i].sign == false ∨ c.lits[i].rhs == mkConst ``False then
+      return [i]
+  return []
+
+def litSelectedOrNothingSelected (c : MClause) (i : Nat) :=
+  let sel := getSelections c
+  if sel == []
+  then true
+  else sel.contains i
+
+end Duper
