git/abentkamp/duper/Duper/Simp.lean
@@ -1,0 +1,60 @@
+import Duper.ProverM
+import Duper.RuleM
+import Duper.MClause
+import Duper.Util.Iterate
+
+namespace Duper
+open RuleM
+open ProverM
+
+inductive SimpResult (α : Type)
+| Applied (c : α) : SimpResult α
+| Unapplicable : SimpResult α
+| Removed : SimpResult α
+
+namespace SimpResult
+
+def mapM [Monad m] (f : α → m β): SimpResult α → m (SimpResult β)
+| Applied c    => return Applied (← f c)
+| Unapplicable => return Unapplicable
+| Removed      => return Removed
+
+def forM {m : Type u → Type v} [Monad m] {α : Type} (r : SimpResult α) (f : α → m PUnit) : m PUnit :=
+match r with
+| Applied c    => f c
+| Unapplicable => return PUnit.unit
+| Removed      => return PUnit.unit
+
+end SimpResult
+
+open SimpResult
+
+abbrev MSimpRule := MClause → RuleM (SimpResult (List (MClause × Option ProofReconstructor)))
+abbrev SimpRule := Clause → ProverM (SimpResult Clause)
+    
+
+def MSimpRule.toSimpRule (rule : MSimpRule) (ruleName : String)
+    : SimpRule := fun givenClause => do
+  -- Run the rule
+  let (res, cs) ← runSimpRule do
+    let mclause ← loadClause givenClause
+    let cs? ← rule mclause
+    cs?.forM fun cs => do
+      for (c, mkProof) in cs do yieldClause c ruleName mkProof
+    return cs?
+  match res with
+  | Removed           => return Removed
+  | Unapplicable      => return Unapplicable
+  | Applied []        => return Removed
+  | Applied _ => do
+    -- Return first clause, add others to passive set
+    for i in [:cs.size] do
+      let (c, proof) := cs[i]
+      if i == 0 then
+        let _ ← addNewClause c proof
+      else
+        addNewToPassive c proof
+    return Applied cs[0].1
+
+
+end Duper
