git/abentkamp/duper/Duper/Tactic.lean
@@ -1,0 +1,126 @@
+import Lean
+import Duper.Saturate
+import Duper.Unif
+
+open Lean
+open Lean.Meta
+open Duper
+open ProverM
+
+
+namespace Lean.Elab.Tactic
+
+partial def printProof (state : ProverM.State) : TacticM Unit := do
+  Core.checkMaxHeartbeats "printProof"
+  let rec go c (hm : Array (Nat × Clause) := {}) : TacticM Unit := do
+    let info ← getClauseInfo! c
+    if hm.contains (info.number, c) then throwError "Loop! {hm} {info.number}"
+    let hm := hm.push (info.number, c)
+    let parentInfo ← info.proof.parents.mapM (fun pp => getClauseInfo! pp.clause) 
+    let parentIds := parentInfo.map fun info => info.number
+    trace[Prover.debug] "Clause #{info.number} (by {info.proof.ruleName} {parentIds}): {c}"
+    for proofParent in info.proof.parents do
+      go proofParent.clause hm
+  go Clause.empty
+where 
+  getClauseInfo! (c : Clause) : TacticM ClauseInfo := do
+    let some ci := state.allClauses.find? c
+      | throwError "clause info not found: {c}"
+    return ci
+
+def getClauseInfo! (state : ProverM.State) (c : Clause) : TacticM ClauseInfo := do
+  let some ci := state.allClauses.find? c
+    | throwError "clause info not found: {c}"
+  return ci
+
+partial def mkList (state : ProverM.State) (c : Clause) (acc : List Clause := []) : TacticM (List Clause) := do
+  Core.checkMaxHeartbeats "mkList"
+  let info ← getClauseInfo! state c
+  let mut acc := acc
+  -- recursive calls
+  acc := c :: acc
+  for proofParent in info.proof.parents do
+    acc ← mkList state proofParent.clause acc
+  return acc
+
+partial def mkProof (state : ProverM.State) : List Clause → TacticM (List Expr)
+| [] => return []
+| c :: cs => do
+  Core.checkMaxHeartbeats "mkProof"
+  let info ← getClauseInfo! state c
+  let newTarget := c.toForallExpr
+  let mut parents := #[]
+  for parent in info.proof.parents do
+    let number := (← getClauseInfo! state parent.clause).number
+    parents := parents.push ((← getLCtx).findFromUserName? (Name.mkNum `goal number)).get!.toExpr
+  let mut lctx ← getLCtx
+  let mut skdefs : List Expr := []
+  for (fvarId, mkSkProof) in info.proof.introducedSkolems do
+    trace[Meta.debug] "Reconstructing skolems {mkFVar fvarId}"
+    let ty := (state.lctx.get! fvarId).type
+    trace[Meta.debug] "Reconstructing skolems {toString ty}"
+    let userName := (state.lctx.get! fvarId).userName
+    -- let skdef ← mkSorry ty (synthetic := true)
+    let skdef ← mkSkProof parents
+    skdefs := skdef :: skdefs
+    lctx := lctx.mkLetDecl fvarId userName ty skdef
+  let (newProof, otherProofs) ← withLCtx lctx (← getLocalInstances) do
+    trace[Meta.debug] "Reconstructing proof for #{info.number}: {c}"
+    let newProof ← info.proof.mkProof parents info.proof.parents c
+    let otherProofs ←
+      withLetDecl (Name.mkNum `goal info.number) newTarget newProof fun g => do
+        let otherProofs ← mkProof state cs
+        let otherProofs ← otherProofs.mapM fun otherProof => do
+          let mut otherProof ← mkLambdaFVars (usedLetOnly := false) #[g] otherProof
+          for (fvarId, _) in info.proof.introducedSkolems do
+            otherProof ← mkLambdaFVars (usedLetOnly := false) #[mkFVar fvarId] otherProof
+          return otherProof
+        return otherProofs
+    return (newProof, otherProofs)
+  -- trace[Meta.debug] "{newProof :: otherProofs}"
+  return newProof :: otherProofs
+
+def applyProof (state : ProverM.State) : TacticM Unit := do
+  let l ← mkList state Clause.empty
+  trace[Meta.debug] "{l}"
+  let proofs ← mkProof state l
+  assignExprMVar (← getMainGoal) proofs.reverse.head! -- TODO: List.last?
+
+def collectAssumptions : TacticM (Array (Expr × Expr)) := do
+  let mut formulas := #[]
+  for fVarId in (← getLCtx).getFVarIds do
+    let ldecl ← getLocalDecl fVarId
+    unless ldecl.binderInfo.isAuxDecl ∨ not (← inferType ldecl.type).isProp do
+      formulas := formulas.push (← instantiateMVars ldecl.type, ← mkAppM ``eq_true #[mkFVar fVarId])
+  return formulas
+
+syntax (name := duper) "duper" : tactic
+
+@[tactic duper]
+def evalDuper : Tactic
+| `(tactic| duper) => withMainContext do
+  let startTime ← IO.monoMsNow
+  replaceMainGoal [(← intros (← getMainGoal)).2]
+  let mvar ← withMainContext do mkFreshExprMVar (← mkArrow (← mkAppM ``Not #[← getMainTarget]) (mkConst ``False))
+  assignExprMVar (← getMainGoal) (mkApp2 (mkConst ``Classical.byContradiction) (← getMainTarget) mvar)
+  replaceMainGoal [mvar.mvarId!]
+  replaceMainGoal [(← intro (← getMainGoal) `h).2]
+  withMainContext do
+    let formulas ← collectAssumptions
+    trace[Meta.debug] "{formulas}"
+    let (_, state) ← ProverM.runWithExprs (s := {lctx := ← getLCtx}) ProverM.saturate formulas
+    match state.result with
+    | Result.contradiction => do
+        logInfo s!"Contradiction found. Time: {(← IO.monoMsNow) - startTime}ms"
+        printProof state
+        applyProof state
+        logInfo s!"Constructed proof. Time: {(← IO.monoMsNow) - startTime}ms"
+    | Result.saturated => 
+      trace[Prover.debug] "Final Active Set: {state.activeSet.toArray}"
+      -- trace[Prover.debug] "supMainPremiseIdx: {state.supMainPremiseIdx}"
+      throwError "Prover saturated."
+    | Result.unknown => throwError "Prover was terminated."
+| _ => throwUnsupportedSyntax
+
+end Lean.Elab.Tactic
+
