git/abentkamp/duper/Duper/Util/Misc.lean
@@ -1,0 +1,24 @@
+import Lean
+open Lean
+
+instance [Hashable α] : Hashable (Array α) where
+  hash as := as.foldl (fun r a => mixHash r (hash a)) 7
+
+-- TODO: Use this?
+-- #check Lean.Meta.abstractMVars
+
+def Lean.Expr.abstractMVars (e : Expr) (mVars : Array Expr) : Expr :=
+  let rec visit (e : Expr) (offset : Nat) : Expr :=
+    match e with
+    | Expr.mvar .. => 
+      match mVars.indexOf? e with
+      | some i => mkBVar (mVars.size - 1 - i + offset)
+      | none => e
+    | Expr.app f a _       => e.updateApp! (visit f offset) (visit a offset)
+    | Expr.mdata _ b _     => e.updateMData! (visit b offset)
+    | Expr.proj _ _ b _    => e.updateProj! (visit b offset)
+    | Expr.letE _ t v b _  => e.updateLet! (visit t offset) (visit v offset) (visit b (offset+1))
+    | Expr.lam _ d b _     => e.updateLambdaE! (visit d offset) (visit b (offset+1))
+    | Expr.forallE _ d b _ => e.updateForallE! (visit d offset) (visit b (offset+1))
+    | e                    => e
+  visit e 0
