git/abentkamp/duper/Duper/Util/ProofReconstruction.lean
@@ -1,0 +1,53 @@
+import Duper.ProverM
+import Duper.RuleM
+import Duper.MClause
+
+namespace Duper
+open RuleM
+open Lean
+
+def instantiatePremises (parents : Array ProofParent) (premises : Array Expr) (xs : Array Expr) : 
+    MetaM (Array (Array Lit) × Array Expr) := do
+  let mut parentsLits := #[]
+  let mut appliedPremises := #[]
+  for k in [:parents.size] do
+    let vanishingVarSkolems ← parents[k].vanishingVarTypes.mapM fun ty =>
+      Meta.mkAppOptM ``default #[some ty, none]
+    let parentInstantiations := parents[k].instantiations.map (fun ins => ins.instantiateRev (xs ++ vanishingVarSkolems))
+    parentsLits := parentsLits.push $ parents[k].clause.lits.map (fun lit => lit.map (fun e => e.instantiateRev parentInstantiations))
+    appliedPremises := appliedPremises.push $ mkAppN premises[k] parentInstantiations
+  return (parentsLits, appliedPremises)
+
+/-- Construct a proof of `lits[0] ∨ ... ∨ lits[n] → target`, given proofs (`casesProofs`) of `lits[i] → target` -/
+def orCases (lits : Array Expr) (caseProofs : Array Expr) : MetaM Expr := do
+  let mut ors := #[lits[lits.size - 1]]
+  for l in [2:lits.size+1] do
+    ors := ors.push (mkApp2 (mkConst ``Or) lits[lits.size - l] ors[ors.size-1])
+  let mut r := caseProofs[caseProofs.size - 1]
+  for k in [2:caseProofs.size+1] do
+    let newOne := caseProofs[caseProofs.size - k]
+    r ← Meta.withLocalDeclD `h ors[k-1] fun h => do
+      let p ← Meta.mkAppM
+        ``Or.elim
+        #[h, newOne, r]
+      Meta.mkLambdaFVars #[h] p
+  return r
+
+/-- Construct a proof of `lits[0] ∨ ... ∨ lits[n]`, given a `proof` of `lits[i]` -/
+def orIntro (lits : Array Expr) (i : Nat) (proof : Expr) : MetaM Expr := do
+  let mut tyR := lits[lits.size-1]
+  for j in [2:lits.size-i] do
+    tyR := mkApp2 (mkConst ``Or) lits[lits.size - j] tyR
+  let mut proofRight :=
+    if i != lits.size - 1 then
+      mkApp3 (mkConst ``Or.inl) lits[i] tyR proof
+    else
+      proof
+  if i != lits.size - 1 then
+    tyR := mkApp2 (mkConst ``Or) lits[i] tyR
+  for j in [lits.size-i+1:lits.size+1] do
+    proofRight := mkApp3 (mkConst ``Or.inr) lits[lits.size-j] tyR proofRight
+    tyR := mkApp2 (mkConst ``Or) lits[lits.size-j] tyR
+  return proofRight
+
+end Duper
