git/abentkamp/duper/Duper/test.lean
@@ -1,0 +1,147 @@
+import Duper.Tactic
+
+-- set_option trace.Meta.debug true
+-- set_option trace.Prover.saturate true
+-- set_option trace.Prover.debug true
+-- set_option trace.Rule.debug true
+-- set_option pp.all true
+
+constant a : Nat
+constant b : Nat
+constant c : Nat
+constant d : Nat
+constant zero : Nat
+constant one : Nat
+constant div : Nat → Nat → Nat
+constant mul : Nat → Nat → Nat
+constant add : Nat → Nat → Nat
+constant inv : Nat → Nat
+constant f : Nat → Nat
+constant g : Nat → Nat
+constant h : Nat → Nat
+constant p : Nat → Prop
+constant q : Prop
+constant isZero : Nat → Prop
+
+theorem test0000
+(div_self : ∀ x, ¬ isZero x → div x x = one)
+(add_mul : ∀ (x y z : Nat), mul (add x y) z = add (mul x z) (mul y z))
+(div_def : ∀ (x y : Nat), ¬ isZero y → div x y = mul x (inv y)) :
+∀ (x y : Nat), ¬ isZero y → div (add x y) y = add (div x y) one := by duper
+
+-- Contradiction found. Time: 1565ms
+theorem test0018 (a1 a2 a3 a4 a5 a6 : Nat)
+(h1 : 
+f (f (f (f (f (f (f (f a5))))))) = d ∨
+f (f (f (f (f (f (f a4)))))) = d ∨
+f (f (f (f (f (f a3))))) = d ∨
+f (f (f (f (f a2)))) = d ∨
+f (f (f (f a1))) = d ∨
+f (f (f a)) = d ∨ f (f b) = d ∨ f c = d)
+(h2 : f (f (f (f (f (f (f (f a5))))))) ≠ d)
+(h2 : f (f (f (f (f (f (f a4)))))) ≠ d)
+(h2 : f (f (f (f (f (f a3))))) ≠ d)
+(h2 : f (f (f (f (f a2)))) ≠ d)
+(h2 : f (f (f (f a1))) ≠ d)
+(h2 : f (f (f a)) ≠ d)
+(h3 : f (f b) ≠ d)
+(h4 : f c ≠ d)
+: False := by duper
+
+#print test0018
+
+-- theorem test00008
+-- (div_self : ∀ x, x ≠ zero → mul x (inv x) = one)
+-- (add_mul : ∀ (x y z : Nat), mul (add x y) z = add (mul x z) (mul y z)) :
+-- -- (div_def : ∀ (x y : Nat), y ≠ zero → div x y = mul x (inv y)) :
+-- ∀ (x y : Nat), y ≠ zero → mul (add x y) (inv y) = add (mul x (inv y)) one := by duper
+
+
+-- theorem test00008
+-- (div_self : ∀ x, x ≠ zero → div x x = one)
+-- (add_mul : ∀ (x y z : Nat), mul (add x y) z = add (mul x z) (mul y z))
+-- (div_def : ∀ (x y : Nat), y ≠ zero → div x y = mul x (inv y)) :
+-- ∀ (x y : Nat), y ≠ zero → mul (add x y) (inv y) = add (mul x (inv y)) one := by duper
+
+-- #print test
+-- #print axioms test
+
+set_option trace.Prover.debug true
+theorem test 
+(div_self : ∀ x, div x x = one)
+(add_mul : ∀ (x y z : Nat), mul (add x y) z = add (mul x z) (mul y z))
+(div_def : ∀ (x y : Nat), div x y = mul x (inv y)) :
+∀ (x y : Nat), div (add x y) y = add (div x y) one := by duper
+
+#print test
+#print axioms test
+
+-- example --(h : ∃ x, x ≠ c ∨ a = b) 
+-- (h : ¬ ∃ x, x = f a ∨ ∀ x, ∃ y, y = f a ∧ x = b)-- (h :  c = b ∧ a = b) 
+-- : False := by
+--   prover
+--   all_goals
+--     sorry
+#check fun h => Eq.mpr h True.intro
+#check propext
+
+theorem test00
+(ax1 : a ≠ a ∨ ¬ (∀ x : Nat, x = x) ∨ b ≠ b)
+: False := by duper
+
+#print test00
+
+theorem test0
+(ax1 : f a = b → f c ≠ b)
+(ax2 : ¬ ∃ x, f x ≠ b ∧ c = c)
+: False := by duper
+
+#print test0
+
+theorem test1
+(div_self : ∀ x, f x = a)
+(div_self : ∀ x, f x ≠ a)
+: False := by duper
+
+
+#print test1
+
+theorem test1'
+(div_self : ∀ x y z : Nat, f x ≠ f x ∨ g y ≠ g y ∨ h z ≠ h z)
+: False := by duper
+
+theorem test2
+: ∀ (x : Nat), x = x := by duper
+
+#print test2
+
+
+theorem puzzle1 {ι : Type} (johanna : ι) (bill : ι) (peanuts : ι)
+  (food : ι → Prop) (alive : ι → Prop) 
+  (likes : ι → ι → Prop) (eats : ι → ι → Prop) (was_killed_by : ι → ι → Prop)
+  (h1 : ∀ x, food x → likes johanna x)
+  (h2 : ∀ x, (∃ y, eats y x ∧ ¬ was_killed_by y x) → food x)
+  (h3 : eats bill peanuts)
+  (h4 : alive bill)
+  (h5 : ∀ y, alive y → ∀ x, ¬ was_killed_by y x) :
+likes johanna peanuts := by duper
+
+#print puzzle1
+
+#print axioms puzzle1
+-- set_option trace.Meta.debug true
+set_option trace.Prover.saturate true
+-- set_option trace.Prover.debug true
+-- set_option trace.Rule.debug true
+-- set_option pp.all true
+
+-- theorem puzzle2 {ι : Type} (Tarr : ι) (Fether : ι) 
+--   (Doctor : ι → Prop) (Peculiar : ι → Prop) (Sane : ι → Prop)
+--   (bestFriend : ι → ι) (Special : ι → Prop)
+--   (h4 : ∀x, Peculiar x = (Sane x = ¬ Doctor x))
+--   (h5 : ∀x, Special x = (∀y, ¬ Doctor y = (Sane y = Peculiar x)))
+--   (h7 : ∀x, ∀y, (Sane x = Special y) → (Sane (bestFriend x) = ¬ Doctor y))
+--   (h8 : Sane Tarr = ∀x, Doctor x → Sane x)
+--   (h10 : Sane Fether = ∀x, Doctor x → ¬ Sane x)
+--   (h12 : Sane Fether = Sane Tarr) : 
+-- False := by duper
