git/xubaiw/lean-problem-dynamic-link/bar1/Bar1.lean
@@ -1,0 +1,2 @@
+@[export bar1_greet]
+def greet (name : String) := s!"Hello, {name}!"
