git/xubaiw/lean-problem-dynamic-link/bar1/lakefile.lean
@@ -1,0 +1,7 @@
+import Lake
+open Lake DSL
+
+package bar1 {
+  libName := "libbar1"
+  defaultFacet := PackageFacet.sharedLib
+}
