git/xubaiw/lean-problem-dynamic-link/bar2/Main.lean
@@ -1,0 +1,5 @@
+@[extern "bar1_greet"]
+constant greet : String → String
+
+def main : IO Unit :=
+  IO.println <| greet "Lean Programmers"
