git/xubaiw/lean-problem-dynamic-link/bar2/lakefile.lean
@@ -1,0 +1,15 @@
+import Lake
+open System Lake DSL
+
+package bar2 (pkgDir) (args) do
+  let current ← IO.currentDir
+  let dylibDir := current / ".." / "bar1" / "build" / "lib" 
+  let dylib := dylibDir / s!"libbar1.{sharedLibExt}"
+  IO.println s!"link to {dylib}"
+  return {
+    name := `bar2
+    moreLibTargets := #[
+      inputFileTarget dylib
+    ]
+    moreLinkArgs := #["-l", "bar1", "-L", dylibDir.toString]
+  }
