git/xubaiw/lean-problem-dynamic-link/README.md
@@ -1,0 +1,55 @@
+# Problems with Lean Dynamic Link 
+
+## How to reproduce the error
+
+```sh
+$ cd bar1
+$ lake build
+...
+$ cd ../bar2
+$ lake build
+...
+$ ./build/bin/bar2  -- running the program produce the error
+dyld[66116]: Library not loaded: ./build/lib/libbar1.dylib
+  Referenced from: /Users/xubaiw/bar/bar2/build/bin/bar2
+  Reason: tried: './build/lib/libbar1.dylib' (no such file), '/usr/local/lib/libbar1.dylib' (no such file), '/usr/lib/libbar1.dylib' (no such file), '/Users/xubaiw/bar/bar2/build/lib/libbar1.dylib' (no such file), '/usr/local/lib/libbar1.dylib' (no such file), '/usr/lib/libbar1.dylib' (no such file)
+zsh: abort      ./build/bin/bar2
+```
+
+## Details
+
+In this repo we have two lean packages: `bar1` and `bar2`.
+
+In `bar1` there is:
+
+```lean
+@[export bar1_greet]
+def greet (name : String) := s!"Hello, {name}!"
+```
+
+Then `bar1` is compiled to  a sharedLib. In order to use the definition, in `bar2` we have:
+
+```lean
+@[extern "bar1_greet"]
+constant greet : String → String
+
+def main : IO Unit :=
+  IO.println <| greet "Lean Programmers"
+```
+
+Both `moreLibTargets` and `moreLinkArgs` is used in `bar2`:
+
+```lean
+package bar2 (pkgDir) (args) do
+  let current ← IO.currentDir
+  let dylibDir := current / ".." / "bar1" / "build" / "lib" 
+  let dylib := dylibDir / s!"libbar1.{sharedLibExt}"
+  IO.println s!"link to {dylib}"
+  return {
+    name := `bar2
+    moreLibTargets := #[
+      inputFileTarget dylib
+    ]
+    moreLinkArgs := #["-l", "bar1", "-L", dylibDir.toString]
+  }
+```
